String matrix changed to sequences, accessing matrix elements no good in Dafny.

dp/lcs.dfy
@@ -11,40 +11,38 @@ reads a
                     ==> a[i, j] == 0 
 }
 
-predicate leftPaddedDimMatrix(a: array2<char>, b: array2<nat>)
-requires 0 < a.Length0 && 0 < a.Length1
-reads a
+predicate leftPaddedDimMatrix(s1: seq<char>, s2: seq<char>, b: array2<nat>)
+requires 0 < |s1| && 0 < |s2|
 {
-    b.Length0 == a.Length0 && b.Length1 == a.Length1 
-    && a[0, 0] == '\0' 
+    b.Length0 == |s1| && b.Length1 == |s2|
+    && s2[0] == s1[0] == '\0' 
 }
 
-function recLCS(a: array2<char>, i: int, j: int): nat
-reads a
+function recLCS(s1: seq<char>, s2: seq<char>, i: int, j: int): nat
 decreases i, j
-requires 0 <= i < a.Length0
-requires 0 <= j < a.Length1
+requires 0 <= i < |s1|
+requires 0 <= j < |s2|
 {
     if i == 0 || j == 0
         then 0
-    else if a[i, j] != a[i, j]
-        then if recLCS(a, i-1, j) > recLCS(a, i, j-1)
-            then recLCS(a, i-1, j)
-            else recLCS(a, i, j-1)
-        else if a[i, j] == a[i, j]
-            then if recLCS(a, i-1, j) > recLCS(a, i, j-1) && recLCS(a, i-1, j) > 1 + recLCS(a, i-1, j-1)
-                then recLCS(a, i-1, j)
-                else if recLCS(a, i, j-1) > recLCS(a, i-1, j) && recLCS(a, i, j-1) > 1 + recLCS(a, i-1, j-1)
-                    then recLCS(a, i, j-1)
-                    else 1 + recLCS(a, i-1, j-1)
+    else if s1[i] != s2[j]
+        then if recLCS(s1, s2, i-1, j) > recLCS(s1, s2, i, j-1)
+            then recLCS(s1, s2, i-1, j)
+            else recLCS(s1, s2, i, j-1)
+        else if s1[i] == s2[j]
+            then if recLCS(s1, s2, i-1, j) > recLCS(s1, s2, i, j-1) && recLCS(s1, s2, i-1, j) > 1 + recLCS(s1, s2, i-1, j-1)
+                then recLCS(s1, s2, i-1, j)
+                else if recLCS(s1, s2, i, j-1) > recLCS(s1, s2, i-1, j) && recLCS(s1, s2, i, j-1) > 1 + recLCS(s1, s2, i-1, j-1)
+                    then recLCS(s1, s2, i, j-1)
+                    else 1 + recLCS(s1, s2, i-1, j-1)
             else 0
 }
 
-method dpLCS(s: array2<char>, lcsMatrix: array2<nat>) returns (lcsLen: nat)
-requires 0 < lcsMatrix.Length0 == s.Length0 && 0 < lcsMatrix.Length1 == s.Length1
+method dpLCS(s1: seq<char>, s2: seq<char>, lcsMatrix: array2<nat>) returns (lcsLen: nat)
+requires 0 < lcsMatrix.Length0 == |s1| && 0 < lcsMatrix.Length1 == |s2|
 requires rowColInitializedMatrix(lcsMatrix)
-requires leftPaddedDimMatrix(s, lcsMatrix)
-ensures s.Length0-1 > 0 && s.Length1-1 > 0 ==> lcsLen == recLCS(s, s.Length0-1, s.Length1-1)
+requires leftPaddedDimMatrix(s1, s2, lcsMatrix)
+ensures |s1|-1 > 0 && |s2|-1 > 0 ==> lcsLen == recLCS(s1, s2, |s1|-1, |s2|-1)
 {
     var rowLen, colLen := lcsMatrix.Length0, lcsMatrix.Length1;
     var i, j := 1, 1;
@@ -64,5 +62,5 @@ ensures s.Length0-1 > 0 && s.Length1-1 > 0 ==> lcsLen == recLCS(s, s.Length0-1, 
         i := i + 1;
     }
 
-    assume s.Length0-1 > 0 && s.Length1-1 > 0 ==> lcsLen == recLCS(s, s.Length0-1, s.Length1-1);
+    assume |s1|-1 > 0 && |s2|-1 > 0 ==> lcsLen == recLCS(s1, s2, |s1|-1, |s2|-1);
 }
